lunarlander_sl/BigStepSimple.thy
@@ -4,77 +4,18 @@ begin
 
 subsection \<open>Syntax\<close>
 
-text \<open>State\<close>
-type_synonym state = "char \<Rightarrow> real"
-
-text \<open>Expressions\<close>
-type_synonym exp = "state \<Rightarrow> real"
-
-text \<open>Predicates\<close>
-type_synonym fform = "state \<Rightarrow> bool"
-
 text \<open>Channel names\<close>
 type_synonym cname = string
-
-text \<open>Time\<close>
-type_synonym time = real
-
-text \<open>Variable names\<close>
-type_synonym var = char
-
-text \<open>Some common variables\<close>
-definition X :: char where "X = CHR ''x''"
-definition Y :: char where "Y = CHR ''y''"
-definition Z :: char where "Z = CHR ''z''"
-
-lemma vars_distinct [simp]: "X \<noteq> Y" "X \<noteq> Z" "Y \<noteq> Z" "Y \<noteq> X" "Z \<noteq> X" "Z \<noteq> Y"
-  unfolding X_def Y_def Z_def by auto
 
 text \<open>Ready information.
   First component is set of channels that are ready to output.
   Second component is set of channels that are ready to input.\<close>
 type_synonym rdy_info = "cname set \<times> cname set"
 
-text \<open>History at a time interval\<close>
-type_synonym history = "time \<Rightarrow> state"
-
 text \<open>Communications\<close>
 datatype comm =
-  Send cname exp         ("_[!]_" [110,108] 100)
+  Send cname exp        ("_[!]_" [110,108] 100)
 | Receive cname var     ("_[?]_" [110,108] 100)
-
-text \<open>Definition of ODEs\<close>
-
-type_synonym vec = "real^(var)"
-
-text \<open>Conversion between state and vector\<close>
-definition state2vec :: "state \<Rightarrow> vec" where
-  "state2vec s = (\<chi> x. s x)"
-
-definition vec2state :: "vec \<Rightarrow> state" where
-  "(vec2state v) x = v $ x"
-
-lemma vec_state_map1[simp]: "vec2state (state2vec s) = s"
-  unfolding vec2state_def state2vec_def by auto
-
-lemma vec_state_map2[simp]: "state2vec (vec2state s) = s"
-  unfolding vec2state_def state2vec_def by auto
-
-datatype ODE =
-  ODE "var \<Rightarrow> exp"
-
-text \<open>Given ODE and a state, find the derivative vector.\<close>
-fun ODE2Vec :: "ODE \<Rightarrow> state \<Rightarrow> vec" where
-  "ODE2Vec (ODE f) s = state2vec (\<lambda>a. f a s)"
-
-text \<open>History p on time {0 .. d} is a solution to ode.\<close>
-definition ODEsol :: "ODE \<Rightarrow> (real \<Rightarrow> state) \<Rightarrow> real \<Rightarrow> bool" where
-  "ODEsol ode p d = (d \<ge> 0 \<and> (((\<lambda>t. state2vec (p t)) has_vderiv_on (\<lambda>t. ODE2Vec ode (p t))) {0 .. d}))"
-
-text \<open>History p on time {0 ..} is a solution to ode.\<close>
-definition ODEsolInf :: "ODE \<Rightarrow> (real \<Rightarrow> state) \<Rightarrow> bool" where
-  "ODEsolInf ode p = (((\<lambda>t. state2vec (p t)) has_vderiv_on (\<lambda>t. ODE2Vec ode (p t))) {0 ..})"
-
 
 text \<open>HCSP processes\<close>
 datatype proc =
@@ -83,7 +24,7 @@ datatype proc =
 | Assign var exp             ("_ ::= _" [99,95] 94)
 | Seq proc proc           ("_; _" [91,90] 90)
 | Cond fform proc proc        ("IF _ _ _" [95,94] 93)
-| Wait time  \<comment> \<open>Waiting for a specified amount of time\<close>
+| Wait real  \<comment> \<open>Waiting for a specified amount of time\<close>
 | IChoice proc proc  \<comment> \<open>Nondeterminism\<close>
 | EChoice "(comm \<times> proc) list"  \<comment> \<open>External choice\<close>
 | Rep proc   \<comment> \<open>Nondeterministic repetition\<close>
@@ -95,12 +36,6 @@ datatype pproc =
   Single proc
 | Parallel pproc "cname set" pproc
 
-text \<open>Events\<close>
-datatype event =
-  In cname real
-| Out cname real 
-| IO cname real 
-
 text \<open>Global states\<close>
 datatype gstate =
   State state
@@ -108,13 +43,11 @@ datatype gstate =
 
 subsection \<open>Traces\<close>
 
-text \<open>First, we define the concept of traces\<close>
-
 datatype trace_block =
   InBlock cname real
   | OutBlock cname real
   | IOBlock cname real
-  | WaitBlock time "real \<Rightarrow> gstate" rdy_info
+  | WaitBlock real "real \<Rightarrow> gstate" rdy_info
 
 type_synonym trace = "trace_block list"
 
@@ -126,10 +59,10 @@ subsection \<open>Big-step semantics\<close>
 text \<open>Compute list of ready communications for an external choice.\<close>
 fun rdy_of_echoice :: "(comm \<times> proc) list \<Rightarrow> rdy_info" where
   "rdy_of_echoice [] = ({}, {})"
-| "rdy_of_echoice ((Send ch e, _) # rest) = (
+| "rdy_of_echoice ((ch[!]e, _) # rest) = (
     let rdy = rdy_of_echoice rest in
       (insert ch (fst rdy), snd rdy))"
-| "rdy_of_echoice ((Receive ch var, _) # rest) = (
+| "rdy_of_echoice ((ch[?]var, _) # rest) = (
     let rdy = rdy_of_echoice rest in
       (fst rdy, insert ch (snd rdy)))"
 
@@ -140,9 +73,9 @@ inductive big_step :: "proc \<Rightarrow> state \<Rightarrow> trace \<Rightarrow
 | assignB: "big_step (var ::= e) s [] (s(var := e s))"
 | seqB: "big_step p1 s1 tr1 s2 \<Longrightarrow>
          big_step p2 s2 tr2 s3 \<Longrightarrow>
-         big_step (Seq p1 p2) s1 (tr1 @ tr2) s3"
-| condB1: "b s1 \<Longrightarrow> big_step p1 s1 tr s2 \<Longrightarrow> big_step (Cond b p1 p2) s1 tr s2"
-| condB2: "\<not> b s1 \<Longrightarrow> big_step p2 s1 tr s2 \<Longrightarrow> big_step (Cond b p1 p2) s1 tr s2"
+         big_step (p1; p2) s1 (tr1 @ tr2) s3"
+| condB1: "b s1 \<Longrightarrow> big_step p1 s1 tr s2 \<Longrightarrow> big_step (IF b p1 p2) s1 tr s2"
+| condB2: "\<not> b s1 \<Longrightarrow> big_step p2 s1 tr s2 \<Longrightarrow> big_step (IF b p1 p2) s1 tr s2"
 | waitB1: "d > 0 \<Longrightarrow> big_step (Wait d) s [WaitBlock d (\<lambda>\<tau>\<in>{0..d}. State s) ({}, {})] s"
 | waitB2: "\<not> d > 0 \<Longrightarrow> big_step (Wait d) s [] s"
 | sendB1: "big_step (Cm (ch[!]e)) s [OutBlock ch (e s)] s"
@@ -205,36 +138,26 @@ inductive big_step :: "proc \<Rightarrow> state \<Rightarrow> trace \<Rightarrow
     rdy = rdy_of_echoice cs \<Longrightarrow>
     big_step (Interrupt ode b cs) s1 [WaitBlock d (\<lambda>\<tau>\<in>{0..d}. State (p \<tau>)) rdy] s2"
 
+lemma big_step_cong:
+  "big_step c s1 tr s2 \<Longrightarrow> tr = tr' \<Longrightarrow> s2 = s2' \<Longrightarrow> big_step c s1 tr' s2'"
+  by auto
 
-subsection \<open>More convenient version of rules\<close>
-
-lemma assignB':
-  assumes "s2 = s1(var := e s1)"
-  shows "big_step (Assign var e) s1 [] s2"
-  unfolding assms by (rule assignB)
-
-lemma sendB1':
-  assumes "blks = [OutBlock ch (e s)]"
-  shows "big_step (Cm (Send ch e)) s blks s"
-  unfolding assms by (rule sendB1)
-
-lemma seqB':
-  assumes "big_step p1 s1 tr1 s2"
-    and "big_step p2 s2 tr2 s3"
-    and "tr = tr1 @ tr2"
-  shows "big_step (p1; p2) s1 tr s3"
-  unfolding assms(3) using assms(1-2) by (rule seqB)
-
-lemma receiveB2':
-  assumes "d > 0"
-    and "blks = [WaitBlock d (\<lambda>\<tau>\<in>{0..d}. State s) ({}, {ch}),
-                 InBlock ch v]"
-    and "s' = s(var := v)"
-  shows "big_step (Cm (ch[?]var)) s blks s'"
-  unfolding assms(2-3) using assms(1) by (rule receiveB2)
+inductive_cases skipE: "big_step Skip s1 tr s2"
+inductive_cases assignE: "big_step (Assign var e) s1 tr s2"
+inductive_cases sendE: "big_step (Cm (ch[!]e)) s1 tr s2"
+inductive_cases receiveE: "big_step (Cm (ch[?]var)) s1 tr s2"
+inductive_cases seqE: "big_step (Seq p1 p2) s1 tr s2"
+inductive_cases condE: "big_step (Cond b p1 p2) s1 tr s2"
+inductive_cases waitE: "big_step (Wait d) s1 tr s2"
+inductive_cases echoiceE: "big_step (EChoice es) s1 tr s2"
+inductive_cases ichoiceE: "big_step (IChoice p1 p2) s1 tr s2"
+inductive_cases contE: "big_step (Cont ode b) s1 tr s2"
+inductive_cases interruptE: "big_step (Interrupt ode b cs) s1 tr s2"
 
 
 subsection \<open>Validity\<close>
+
+text \<open>Assertion is a predicate on states and traces\<close>
 
 type_synonym assn = "state \<Rightarrow> trace \<Rightarrow> bool"
 
@@ -263,39 +186,6 @@ lemma Valid_ex_post:
 lemma Valid_and_pre:
   "(P1 \<Longrightarrow> Valid P c Q) \<Longrightarrow> Valid (\<lambda>s t. P1 \<and> P s t) c Q"
   unfolding Valid_def by auto
-
-inductive_cases skipE: "big_step Skip s1 tr s2"
-thm skipE
-
-inductive_cases assignE: "big_step (Assign var e) s1 tr s2"
-thm assignE
-
-inductive_cases sendE: "big_step (Cm (ch[!]e)) s1 tr s2"
-thm sendE
-
-inductive_cases receiveE: "big_step (Cm (ch[?]var)) s1 tr s2"
-thm receiveE
-
-inductive_cases seqE: "big_step (Seq p1 p2) s1 tr s2"
-thm seqE
-
-inductive_cases condE: "big_step (Cond b p1 p2) s1 tr s2"
-thm condE
-
-inductive_cases waitE: "big_step (Wait d) s1 tr s2"
-thm waitE
-
-inductive_cases echoiceE: "big_step (EChoice es) s1 tr s2"
-thm echoiceE
-
-inductive_cases ichoiceE: "big_step (IChoice p1 p2) s1 tr s2"
-thm ichoiceE
-
-inductive_cases contE: "big_step (Cont ode b) s1 tr s2"
-thm contE
-
-inductive_cases interruptE: "big_step (Interrupt ode b cs) s1 tr s2"
-thm interruptE
 
 theorem Valid_weaken_pre:
   "P \<Longrightarrow>\<^sub>A P' \<Longrightarrow> Valid P' c Q \<Longrightarrow> Valid P c Q"
@@ -461,49 +351,7 @@ proof -
 qed
 
 
-text \<open>Some special cases of EChoice\<close>
-
-lemma InIn_lemma:
-  assumes "Q ch1 var1 p1"
-    and "Q ch2 var2 p2"
-    and "i < length [(ch1[?]var1, p1), (ch2[?]var2, p2)]"
-  shows "case [(ch1[?]var1, p1), (ch2[?]var2, p2)] ! i of
-            (ch[!]e, p1) \<Rightarrow> P ch e p1
-          | (ch[?]var, p1) \<Rightarrow> Q ch var p1"
-proof -
-  have "case comm of ch[!]e \<Rightarrow> P ch e p | ch[?]var \<Rightarrow> Q ch var p"
-    if "i < Suc (Suc 0)"
-       "[(ch1[?]var1, p1), (ch2[?]var2, p2)] ! i = (comm, p)" for comm p i
-  proof -
-    have "i = 0 \<or> i = 1"
-      using that(1) by auto
-    then show ?thesis
-      apply (rule disjE)
-      using that(2) assms by auto
-  qed
-  then show ?thesis
-    using assms(3) by auto
-qed
-
-theorem Valid_echoice_InIn:
-  assumes "Valid Q1 p1 R"
-    and "Valid Q2 p2 R"
-  shows "Valid
-    (\<lambda>s tr. (\<forall>v. Q1 (s(var1 := v)) (tr @ [InBlock ch1 v])) \<and>
-            (\<forall>d>0. \<forall>v. Q1 (s(var1 := v)) (tr @ [WaitBlock d (\<lambda>\<tau>\<in>{0..d}. State s) ({}, {ch1, ch2}), InBlock ch1 v])) \<and>
-            (\<forall>v. Q2 (s(var2 := v)) (tr @ [InBlock ch2 v])) \<and>
-            (\<forall>d>0. \<forall>v. Q2 (s(var2 := v)) (tr @ [WaitBlock d (\<lambda>\<tau>\<in>{0..d}. State s) ({}, {ch1, ch2}), InBlock ch2 v])))
-      (EChoice [(ch1[?]var1, p1), (ch2[?]var2, p2)])
-    R"
-  apply (rule Valid_echoice)
-  apply (rule InIn_lemma)
-  subgoal apply (rule exI[where x=Q1])
-    by (auto simp add: assms entails_def)
-  apply (rule exI[where x=Q2])
-  by (auto simp add: assms entails_def)
-
-
-subsection \<open>Standard assertions\<close>
+subsection \<open>Assertions on traces\<close>
 
 definition entails_tassn :: "tassn \<Rightarrow> tassn \<Rightarrow> bool" (infixr "\<Longrightarrow>\<^sub>t" 25) where
   "(P \<Longrightarrow>\<^sub>t Q) \<longleftrightarrow> (\<forall>tr. P tr \<longrightarrow> Q tr)"
@@ -524,11 +372,8 @@ lemma entails_tassn_ex_post:
   "(\<exists>x. P \<Longrightarrow>\<^sub>t Q x) \<Longrightarrow> P \<Longrightarrow>\<^sub>t (\<lambda>tr. (\<exists>x. Q x tr))"
   by (auto simp add: entails_tassn_def)
 
-definition and_assn :: "tassn \<Rightarrow> tassn \<Rightarrow> tassn" (infixr "\<and>\<^sub>A" 35) where
-  "(P \<and>\<^sub>A Q) = (\<lambda>tr. P tr \<and> Q tr)"
-
-definition emp_assn :: "tassn" ("emp\<^sub>A") where
-  "emp\<^sub>A = (\<lambda>tr. tr = [])"
+definition emp_assn :: "tassn" ("emp\<^sub>t") where
+  "emp\<^sub>t = (\<lambda>tr. tr = [])"
 
 definition join_assn :: "tassn \<Rightarrow> tassn \<Rightarrow> tassn" (infixr "@\<^sub>t" 65) where
   "P @\<^sub>t Q = (\<lambda>tr. \<exists>tr1 tr2. P tr1 \<and> Q tr2 \<and> tr = tr1 @ tr2)"
@@ -536,8 +381,8 @@ definition join_assn :: "tassn \<Rightarrow> tassn \<Rightarrow> tassn" (infixr 
 definition magic_wand_assn :: "tassn \<Rightarrow> tassn \<Rightarrow> tassn" (infixr "@-" 65) where
   "Q @- P = (\<lambda>tr. \<forall>tr1. Q tr1 \<longrightarrow> P (tr @ tr1))"
 
-definition all_assn :: "(real \<Rightarrow> tassn) \<Rightarrow> tassn" (binder "\<forall>\<^sub>A" 10) where
-  "(\<forall>\<^sub>A v. P v) = (\<lambda>tr. \<forall>v. P v tr)"
+definition all_assn :: "(real \<Rightarrow> tassn) \<Rightarrow> tassn" (binder "\<forall>\<^sub>t" 10) where
+  "(\<forall>\<^sub>tv. P v) = (\<lambda>tr. \<forall>v. P v tr)"
 
 definition conj_assn :: "tassn \<Rightarrow> tassn \<Rightarrow> tassn" (infixr "\<and>\<^sub>t" 35) where
   "(P \<and>\<^sub>t Q) = (\<lambda>tr. P tr \<and> Q tr)"
@@ -548,28 +393,28 @@ definition disj_assn :: "tassn \<Rightarrow> tassn \<Rightarrow> tassn" (infixr 
 definition pure_assn :: "bool \<Rightarrow> tassn" ("\<up>") where
   "\<up>b = (\<lambda>_. b)"
 
-inductive out_assn :: "state \<Rightarrow> cname \<Rightarrow> real \<Rightarrow> tassn" ("Out\<^sub>A") where
-  "Out\<^sub>A s ch v [OutBlock ch v]"
-| "d > 0 \<Longrightarrow> Out\<^sub>A s ch v [WaitBlock d (\<lambda>\<tau>\<in>{0..d}. State s) ({ch}, {}), OutBlock ch v]"
+inductive out_assn :: "state \<Rightarrow> cname \<Rightarrow> real \<Rightarrow> tassn" ("Out\<^sub>t") where
+  "Out\<^sub>t s ch v [OutBlock ch v]"
+| "d > 0 \<Longrightarrow> Out\<^sub>t s ch v [WaitBlock d (\<lambda>\<tau>\<in>{0..d}. State s) ({ch}, {}), OutBlock ch v]"
 
-inductive in_assn :: "state \<Rightarrow> cname \<Rightarrow> real \<Rightarrow> tassn" ("In\<^sub>A") where
-  "In\<^sub>A s ch v [InBlock ch v]"
-| "d > 0 \<Longrightarrow> In\<^sub>A s ch v [WaitBlock d (\<lambda>\<tau>\<in>{0..d}. State s) ({}, {ch}), InBlock ch v]"
+inductive in_assn :: "state \<Rightarrow> cname \<Rightarrow> real \<Rightarrow> tassn" ("In\<^sub>t") where
+  "In\<^sub>t s ch v [InBlock ch v]"
+| "d > 0 \<Longrightarrow> In\<^sub>t s ch v [WaitBlock d (\<lambda>\<tau>\<in>{0..d}. State s) ({}, {ch}), InBlock ch v]"
 
-inductive io_assn :: "cname \<Rightarrow> real \<Rightarrow> tassn" ("IO\<^sub>A") where
-  "IO\<^sub>A ch v [IOBlock ch v]"
+inductive io_assn :: "cname \<Rightarrow> real \<Rightarrow> tassn" ("IO\<^sub>t") where
+  "IO\<^sub>t ch v [IOBlock ch v]"
 
-inductive wait_assn :: "real \<Rightarrow> (real \<Rightarrow> gstate) \<Rightarrow> rdy_info \<Rightarrow> tassn" ("Wait\<^sub>A") where
-  "Wait\<^sub>A d p rdy [WaitBlock d (\<lambda>\<tau>\<in>{0..d}. p \<tau>) rdy]"
+inductive wait_assn :: "real \<Rightarrow> (real \<Rightarrow> gstate) \<Rightarrow> rdy_info \<Rightarrow> tassn" ("Wait\<^sub>t") where
+  "Wait\<^sub>t d p rdy [WaitBlock d (\<lambda>\<tau>\<in>{0..d}. p \<tau>) rdy]"
 
-abbreviation "WaitS\<^sub>A d p \<equiv> Wait\<^sub>A d (\<lambda>t. State (p t))"
+abbreviation "WaitS\<^sub>t d p \<equiv> Wait\<^sub>t d (\<lambda>t. State (p t))"
 
 lemma emp_unit_left [simp]:
-  "(emp\<^sub>A @\<^sub>t P) = P"
+  "(emp\<^sub>t @\<^sub>t P) = P"
   unfolding join_assn_def emp_assn_def by auto
 
 lemma emp_unit_right [simp]:
-  "(P @\<^sub>t emp\<^sub>A) = P"
+  "(P @\<^sub>t emp\<^sub>t) = P"
   unfolding join_assn_def emp_assn_def by auto
 
 lemma join_assoc:
@@ -577,7 +422,7 @@ lemma join_assoc:
   unfolding join_assn_def by fastforce
 
 lemma entails_mp_emp:
-  "emp\<^sub>A \<Longrightarrow>\<^sub>t P @- P"
+  "emp\<^sub>t \<Longrightarrow>\<^sub>t P @- P"
   unfolding entails_tassn_def emp_assn_def magic_wand_assn_def by auto
 
 lemma entails_mp:
@@ -603,9 +448,11 @@ lemma entails_tassn_cancel_left:
   "Q \<Longrightarrow>\<^sub>t R \<Longrightarrow> P @\<^sub>t Q \<Longrightarrow>\<^sub>t P @\<^sub>t R"
   by (auto simp add: entails_tassn_def join_assn_def)
 
+text \<open>Simpler forms of weakest precondition\<close>
+
 theorem Valid_send':
   "Valid
-    (\<lambda>s. Out\<^sub>A s ch (e s) @- Q s)
+    (\<lambda>s. Out\<^sub>t s ch (e s) @- Q s)
     (Cm (ch[!]e))
     Q"
   apply (rule Valid_weaken_pre)
@@ -615,7 +462,7 @@ theorem Valid_send':
 
 theorem Valid_receive':
   "Valid
-    (\<lambda>s. \<forall>\<^sub>A v. In\<^sub>A s ch v @- Q (s(var := v)))
+    (\<lambda>s. \<forall>\<^sub>t v. In\<^sub>t s ch v @- Q (s(var := v)))
     (Cm (ch[?]var))
     Q"
   apply (rule Valid_weaken_pre)
@@ -625,7 +472,7 @@ theorem Valid_receive':
 
 theorem Valid_wait':
   "d > 0 \<Longrightarrow> Valid
-    (\<lambda>s. WaitS\<^sub>A d (\<lambda>_. s) ({}, {}) @- Q s)
+    (\<lambda>s. WaitS\<^sub>t d (\<lambda>_. s) ({}, {}) @- Q s)
     (Wait d)
     Q"
   apply (rule Valid_weaken_pre)
@@ -633,14 +480,7 @@ theorem Valid_wait':
   unfolding entails_def magic_wand_assn_def
   by (auto intro: wait_assn.intros)
 
-theorem Valid_wait_sp:
-  "d > 0 \<Longrightarrow> Valid
-    (\<lambda>s tr. s = st \<and> P s tr)
-    (Wait d)
-    (\<lambda>s tr. s = st \<and> (P s @\<^sub>t WaitS\<^sub>A d (\<lambda>_. st) ({}, {})) tr)"
-  apply (rule Valid_weaken_pre)
-   prefer 2 apply (rule Valid_wait')
-  by (auto simp add: entails_def join_assn_def magic_wand_assn_def)
+text \<open>Strongest postcondition forms\<close>
 
 theorem Valid_assign_sp:
   "Valid
@@ -651,23 +491,11 @@ theorem Valid_assign_sp:
    prefer 2 apply (rule Valid_assign)
   by (auto simp add: entails_def)
 
-theorem Valid_assign_sp':
-  "Valid
-    (\<lambda>s t. \<exists>v. s = st v \<and> P v s t)
-    (Assign x e)
-    (\<lambda>s t. \<exists>v. s = (st v)(x := e (st v)) \<and> P v (st v) t)"
-  apply (rule Valid_ex_pre)
-  subgoal for v
-    apply (rule Valid_ex_post)
-    apply (rule exI[where x=v])
-    by (rule Valid_assign_sp)
-  done
-
 theorem Valid_send_sp:
   "Valid
     (\<lambda>s t. s = st \<and> P s t)
     (Cm (ch[!]e))
-    (\<lambda>s t. s = st \<and> (P st @\<^sub>t Out\<^sub>A st ch (e st)) t)"
+    (\<lambda>s t. s = st \<and> (P st @\<^sub>t Out\<^sub>t st ch (e st)) t)"
   apply (rule Valid_weaken_pre)
    prefer 2 apply (rule Valid_send')
   by (auto simp add: entails_def magic_wand_assn_def join_assn_def)
@@ -676,7 +504,7 @@ theorem Valid_receive_sp:
   "Valid
     (\<lambda>s t. s = st \<and> P s t)
     (Cm (ch[?]var))
-    (\<lambda>s t. \<exists>v. s = st(var := v) \<and> (P st @\<^sub>t In\<^sub>A st ch v) t)"
+    (\<lambda>s t. \<exists>v. s = st(var := v) \<and> (P st @\<^sub>t In\<^sub>t st ch v) t)"
   apply (rule Valid_weaken_pre)
    prefer 2 apply (rule Valid_receive)
   unfolding entails_def
@@ -691,29 +519,38 @@ theorem Valid_receive_sp:
     by (simp add: in_assn.intros)
   done
 
-
+theorem Valid_wait_sp:
+  "d > 0 \<Longrightarrow> Valid
+    (\<lambda>s tr. s = st \<and> P s tr)
+    (Wait d)
+    (\<lambda>s tr. s = st \<and> (P s @\<^sub>t WaitS\<^sub>t d (\<lambda>_. st) ({}, {})) tr)"
+  apply (rule Valid_weaken_pre)
+   prefer 2 apply (rule Valid_wait')
+  by (auto simp add: entails_def join_assn_def magic_wand_assn_def)
 
 subsection \<open>Rules for internal and external choice\<close>
 
-inductive inrdy_assn :: "state \<Rightarrow> cname \<Rightarrow> real \<Rightarrow> rdy_info \<Rightarrow> tassn" ("Inrdy\<^sub>A") where
-  "Inrdy\<^sub>A s ch v rdy [InBlock ch v]"
-| "d > 0 \<Longrightarrow> Inrdy\<^sub>A s ch v rdy [WaitBlock d (\<lambda>\<tau>\<in>{0..d}. State s) rdy, InBlock ch v]"
+text \<open>Additional assertions\<close>
 
-inductive outrdy_assn :: "state \<Rightarrow> cname \<Rightarrow> real \<Rightarrow> rdy_info \<Rightarrow> tassn" ("Outrdy\<^sub>A") where
-  "Outrdy\<^sub>A s ch v rdy [OutBlock ch v]"
-| "d > 0 \<Longrightarrow> Outrdy\<^sub>A s ch v rdy [WaitBlock d (\<lambda>\<tau>\<in>{0..d}. State s) rdy, OutBlock ch v]"
+inductive inrdy_assn :: "state \<Rightarrow> cname \<Rightarrow> real \<Rightarrow> rdy_info \<Rightarrow> tassn" ("Inrdy\<^sub>t") where
+  "Inrdy\<^sub>t s ch v rdy [InBlock ch v]"
+| "d > 0 \<Longrightarrow> Inrdy\<^sub>t s ch v rdy [WaitBlock d (\<lambda>\<tau>\<in>{0..d}. State s) rdy, InBlock ch v]"
 
-text \<open>First, we restate the rule for Valid_echoice in simpler form\<close>
+inductive outrdy_assn :: "state \<Rightarrow> cname \<Rightarrow> real \<Rightarrow> rdy_info \<Rightarrow> tassn" ("Outrdy\<^sub>t") where
+  "Outrdy\<^sub>t s ch v rdy [OutBlock ch v]"
+| "d > 0 \<Longrightarrow> Outrdy\<^sub>t s ch v rdy [WaitBlock d (\<lambda>\<tau>\<in>{0..d}. State s) rdy, OutBlock ch v]"
+
+text \<open>Simpler form of weakest precondition\<close>
 
 theorem Valid_echoice':
   assumes "\<And>i. i<length es \<Longrightarrow>
     case es ! i of
       (ch[!]e, p2) \<Rightarrow>
         (\<exists>Q. Valid Q p2 R \<and>
-            (P \<Longrightarrow>\<^sub>A (\<lambda>s. Outrdy\<^sub>A s ch (e s) (rdy_of_echoice es) @- Q s)))
+            (P \<Longrightarrow>\<^sub>A (\<lambda>s. Outrdy\<^sub>t s ch (e s) (rdy_of_echoice es) @- Q s)))
     | (ch[?]var, p2) \<Rightarrow>
         (\<exists>Q. Valid Q p2 R \<and>
-            (P \<Longrightarrow>\<^sub>A (\<lambda>s. \<forall>\<^sub>Av. Inrdy\<^sub>A s ch v (rdy_of_echoice es) @- Q (s(var := v)))))"
+            (P \<Longrightarrow>\<^sub>A (\<lambda>s. \<forall>\<^sub>tv. Inrdy\<^sub>t s ch v (rdy_of_echoice es) @- Q (s(var := v)))))"
   shows "Valid P (EChoice es) R"
 proof -
   have 1: "\<exists>Q. Valid Q p R \<and>
@@ -722,7 +559,7 @@ proof -
     if *: "i < length es" "es ! i = (ch[!]e, p)" for i ch e p
   proof -
     from assms obtain Q where
-      Q: "Valid Q p R \<and> (P \<Longrightarrow>\<^sub>A (\<lambda>s. Outrdy\<^sub>A s ch (e s) (rdy_of_echoice es) @- Q s))"
+      Q: "Valid Q p R \<and> (P \<Longrightarrow>\<^sub>A (\<lambda>s. Outrdy\<^sub>t s ch (e s) (rdy_of_echoice es) @- Q s))"
       using * by fastforce
     show ?thesis
       apply (rule exI[where x=Q])
@@ -735,7 +572,7 @@ proof -
     if *: "i < length es" "es ! i = (ch[?]var, p)" for i ch var p
   proof -
     from assms obtain Q where
-      Q: "Valid Q p R \<and> (P \<Longrightarrow>\<^sub>A (\<lambda>s. \<forall>\<^sub>Av. Inrdy\<^sub>A s ch v (rdy_of_echoice es) @- Q (s(var := v))))"
+      Q: "Valid Q p R \<and> (P \<Longrightarrow>\<^sub>A (\<lambda>s. \<forall>\<^sub>tv. Inrdy\<^sub>t s ch v (rdy_of_echoice es) @- Q (s(var := v))))"
       using * by fastforce
     show ?thesis
       apply (rule exI[where x=Q])
@@ -751,65 +588,15 @@ proof -
     done
 qed
 
-theorem Valid_echoice_InIn':
-  assumes "Valid Q1 p1 R"
-    and "Valid Q2 p2 R"
-  shows "Valid
-    (\<lambda>s. (\<forall>\<^sub>Av. ((Inrdy\<^sub>A s ch1 v ({}, {ch1, ch2})) @- Q1 (s(var1 := v)))) \<and>\<^sub>A
-         (\<forall>\<^sub>Av. ((Inrdy\<^sub>A s ch2 v ({}, {ch1, ch2})) @- Q2 (s(var2 := v)))))
-      (EChoice [(ch1[?]var1, p1), (ch2[?]var2, p2)])
-    R"
-  apply (rule Valid_weaken_pre)
-   prefer 2 apply (rule Valid_echoice_InIn[OF assms(1-2)])
-  apply (auto simp add: entails_def magic_wand_assn_def and_assn_def all_assn_def)
-  by (auto simp add: inrdy_assn.intros)
-
-lemma echoice_test1:
-  "Valid
-    (\<lambda>s. (\<forall>\<^sub>Av. ((Inrdy\<^sub>A s ''ch1'' v ({}, {''ch1'', ''ch2''})) @- Q (s(X := v)))) \<and>\<^sub>A
-         (\<forall>\<^sub>Av. ((Inrdy\<^sub>A s ''ch2'' v ({}, {''ch1'', ''ch2''})) @- Q (s(X := v)))))
-    (EChoice [(''ch1''[?]X, Skip), (''ch2''[?]X, Skip)])
-    Q"
-  apply (rule Valid_echoice_InIn')
-   apply (rule Valid_skip)
-  by (rule Valid_skip)
-
-text \<open>Contrast this with the case of internal choice\<close>
-lemma ichoice_test1:
-  "Valid
-    (\<lambda>s. (\<forall>\<^sub>Av. In\<^sub>A s ''ch1'' v @- Q (s(X := v))) \<and>\<^sub>A
-         (\<forall>\<^sub>Av. In\<^sub>A s ''ch2'' v @- Q (s(X := v))))
-    (IChoice (Cm (''ch1''[?]X)) (Cm (''ch2''[?]X)))
-    Q"
-  apply (rule Valid_weaken_pre)
-   prefer 2 apply (rule Valid_ichoice)
-    apply (rule Valid_receive') apply (rule Valid_receive')
-  unfolding entails_def and_assn_def by auto
-
 text \<open>Strongest postcondition form\<close>
-lemma ichoice_test1':
-  "Valid
-    (\<lambda>s tr. s = st \<and> P tr)
-    (IChoice (Cm (''ch1''[?]X)) (Cm (''ch2''[?]X)))
-    (\<lambda>s tr. (\<exists>v. s = st(X := v) \<and> (P @\<^sub>t In\<^sub>A st ''ch1'' v) tr) \<or>
-            (\<exists>v. s = st(X := v) \<and> (P @\<^sub>t In\<^sub>A st ''ch2'' v) tr))"
-  apply (rule Valid_weaken_pre)
-   prefer 2 apply (rule ichoice_test1)
-  apply (auto simp add: entails_def and_assn_def magic_wand_assn_def join_assn_def all_assn_def)
-  subgoal for tr v tr'
-    apply (rule exI[where x=v])
-    apply auto
-    apply (rule exI[where x=tr])
-    by auto
-  done
 
 theorem Valid_echoice_sp:
   assumes "\<And>i. i<length es \<Longrightarrow>
     case es ! i of
       (ch[!]e, p2) \<Rightarrow>
-        Valid (\<lambda>s tr. s = st \<and> (P s @\<^sub>t Outrdy\<^sub>A s ch (e s) (rdy_of_echoice es)) tr) p2 Q
+        Valid (\<lambda>s tr. s = st \<and> (P s @\<^sub>t Outrdy\<^sub>t s ch (e s) (rdy_of_echoice es)) tr) p2 Q
     | (ch[?]var, p2) \<Rightarrow>
-        Valid (\<lambda>s tr. (\<exists>v. s = st(var := v) \<and> (P st @\<^sub>t Inrdy\<^sub>A st ch v (rdy_of_echoice es)) tr)) p2 Q"
+        Valid (\<lambda>s tr. (\<exists>v. s = st(var := v) \<and> (P st @\<^sub>t Inrdy\<^sub>t st ch v (rdy_of_echoice es)) tr)) p2 Q"
   shows "Valid
     (\<lambda>s tr. s = st \<and> P s tr)
     (EChoice es)
@@ -821,110 +608,18 @@ theorem Valid_echoice_sp:
       apply (cases comm)
       subgoal for ch e
         apply auto
-        apply (rule exI[where x="\<lambda>s tr. s = st \<and> (P s @\<^sub>t Outrdy\<^sub>A s ch (e s) (rdy_of_echoice es)) tr"])
+        apply (rule exI[where x="\<lambda>s tr. s = st \<and> (P s @\<^sub>t Outrdy\<^sub>t s ch (e s) (rdy_of_echoice es)) tr"])
         apply auto
         using assms apply fastforce
         by (auto simp add: entails_def join_assn_def magic_wand_assn_def)
       subgoal for ch var
         apply auto
-        apply (rule exI[where x="\<lambda>s tr. (\<exists>v. s = st(var := v) \<and> (P st @\<^sub>t Inrdy\<^sub>A st ch v (rdy_of_echoice es)) tr)"])
+        apply (rule exI[where x="\<lambda>s tr. (\<exists>v. s = st(var := v) \<and> (P st @\<^sub>t Inrdy\<^sub>t st ch v (rdy_of_echoice es)) tr)"])
         apply auto
         using assms apply fastforce
         by (auto simp add: entails_def magic_wand_assn_def join_assn_def all_assn_def)
       done
     done
   done
-
-theorem Valid_echoice_InIn_sp:
-  assumes "Valid (\<lambda>s tr. (\<exists>v. s = st(var1 := v) \<and> (P st @\<^sub>t Inrdy\<^sub>A st ch1 v ({}, {ch1, ch2})) tr)) p1 Q1"
-    and "Valid (\<lambda>s tr. (\<exists>v. s = st(var2 := v) \<and> (P st @\<^sub>t Inrdy\<^sub>A st ch2 v ({}, {ch1, ch2})) tr)) p2 Q2"
-  shows
-   "Valid
-    (\<lambda>s tr. s = st \<and> P s tr)
-    (EChoice [(ch1[?]var1, p1), (ch2[?]var2, p2)])
-    (\<lambda>s tr. Q1 s tr \<or> Q2 s tr)"
-  apply (rule Valid_echoice_sp)
-  apply (rule InIn_lemma)
-  using assms by (auto simp add: Valid_def)
-
-
-subsection \<open>Test for external choice\<close>
-
-text \<open>Strongest postcondition form\<close>
-lemma testEChoice1:
-  "Valid
-    (\<lambda>s tr. s = st \<and> P s tr)
-    (EChoice [(''ch1''[?]X, Y ::= (\<lambda>s. s Y + s X)), (''ch2''[?]X, Y ::= (\<lambda>s. s Y - s X))])
-    (\<lambda>s tr. (\<exists>v. s = st(X := v, Y := st Y + v) \<and> (P st @\<^sub>t Inrdy\<^sub>A st ''ch1'' v ({}, {''ch1'', ''ch2''})) tr) \<or>
-            (\<exists>v. s = st(X := v, Y := st Y - v) \<and> (P st @\<^sub>t Inrdy\<^sub>A st ''ch2'' v ({}, {''ch1'', ''ch2''})) tr))"
-  apply (rule Valid_strengthen_post)
-  prefer 2
-   apply (rule Valid_echoice_InIn_sp)
-    apply (rule Valid_assign_sp')
-   apply (rule Valid_assign_sp')
-  by auto
-
-datatype dir = CH1 | CH2
-
-fun echoice_ex_inv :: "state \<Rightarrow> (dir \<times> real) list \<Rightarrow> tassn" where
-  "echoice_ex_inv st [] = emp\<^sub>A"
-| "echoice_ex_inv st ((CH1, v) # rest) =
-    Inrdy\<^sub>A st ''ch1'' v ({}, {''ch1'', ''ch2''}) @\<^sub>t echoice_ex_inv (st(X := v, Y := st Y + v)) rest"
-| "echoice_ex_inv st ((CH2, v) # rest) =
-    Inrdy\<^sub>A st ''ch2'' v ({}, {''ch1'', ''ch2''}) @\<^sub>t echoice_ex_inv (st(X := v, Y := st Y - v)) rest"
-
-fun last_echoice_ex :: "state \<Rightarrow> (dir \<times> real) list \<Rightarrow> state" where
-  "last_echoice_ex st [] = st"
-| "last_echoice_ex st ((CH1, v) # rest) = last_echoice_ex (st(X := v, Y := st Y + v)) rest"
-| "last_echoice_ex st ((CH2, v) # rest) = last_echoice_ex (st(X := v, Y := st Y - v)) rest"
-
-lemma echoice_ex_inv_snoc [simp]:
-  "echoice_ex_inv st (ins @ [(CH1, v)]) =
-    echoice_ex_inv st ins @\<^sub>t Inrdy\<^sub>A (last_echoice_ex st ins) ''ch1'' v ({}, {''ch1'', ''ch2''}) \<and>
-   echoice_ex_inv st (ins @ [(CH2, v)]) =
-    echoice_ex_inv st ins @\<^sub>t Inrdy\<^sub>A (last_echoice_ex st ins) ''ch2'' v ({}, {''ch1'', ''ch2''})"
-  apply (induct ins arbitrary: st)
-  subgoal by auto
-  apply auto subgoal for dir v ins st
-    apply (cases dir)
-    by (auto simp add: join_assoc)
-  subgoal for dir v ins st
-    apply (cases dir)
-    by (auto simp add: join_assoc)
-  done
-
-lemma last_echoice_ex_snoc [simp]:
-  "last_echoice_ex st (ins @ [(CH1, v)]) = (last_echoice_ex st ins)(X := v, Y := last_echoice_ex st ins Y + v) \<and>
-   last_echoice_ex st (ins @ [(CH2, v)]) = (last_echoice_ex st ins)(X := v, Y := last_echoice_ex st ins Y - v)"
-  apply (induct ins arbitrary: st)
-  apply auto
-  by (metis (full_types) dir.exhaust last_echoice_ex.simps(2) last_echoice_ex.simps(3))+
-
-lemma testEChoice:
-  "Valid
-    (\<lambda>s tr. s = st \<and> tr = [])
-    (Rep (EChoice [(''ch1''[?]X, Y ::= (\<lambda>s. s Y + s X)), (''ch2''[?]X, Y ::= (\<lambda>s. s Y - s X))]))
-    (\<lambda>s tr. \<exists>ins. s = last_echoice_ex st ins \<and> echoice_ex_inv st ins tr)"
-  apply (rule Valid_weaken_pre)
-   prefer 2 apply (rule Valid_rep)
-   apply (rule Valid_ex_pre)
-  subgoal for ins
-    apply (rule Valid_strengthen_post)
-    prefer 2
-     apply (rule Valid_echoice_InIn_sp)
-    apply (rule Valid_assign_sp')
-     apply (rule Valid_assign_sp')
-    apply (auto simp add: entails_def)
-    subgoal for tr v
-      apply (rule exI[where x="ins@[(CH1,v)]"])
-      by auto
-    subgoal for tr v
-      apply (rule exI[where x="ins@[(CH2,v)]"])
-      by auto
-    done
-  apply (auto simp add: entails_def)
-  apply (rule exI[where x="[]"])
-  by (auto simp add: emp_assn_def)
-
 
 end
